model/Temporal.lean
@@ -1,7 +1,3 @@
 import Temporal.API
 import Temporal.DynamicConfig
-import Temporal.Experiment.DSL
-import Temporal.Experiment.Compiler
-import Temporal.Experiment.Json
 import Temporal.Umpire.NexusCallerClosure
-import Temporal.Experiment.SwitchScenario
